compiler/backend/proofs/bvi_to_dataProofScript.sml
@@ -590,6 +590,7 @@ Proof
      \\ Q.EXISTS_TAC `t`
      \\ Cases_on ‘z’ \\ gvs [data_to_bvi_ref_def,data_to_bvi_v_Boolv])
   >- (rename [‘Build parts’]
+      \\ ‘domain t.code = domain r.code’ by fs [code_rel_def]
       \\ pairarg_tac \\ gvs [PULL_EXISTS]
       \\ fs [dataSemTheory.do_build_const_def,bvlSemTheory.do_build_const_def]
       \\ irule do_build_thm
