compiler/backend/semantics/bvlPropsScript.sml
@@ -75,6 +75,7 @@ Theorem do_app_Rval_swap:
           clock := x1.clock; ffi := x1.ffi |>)
 Proof
   rw[do_app_cases_val] \\ rfs[SUBSET_DEF] \\ fs []
+  \\ gvs [EVERY_MEM] \\ rw [] \\ res_tac \\ fs []
 QED
 
 Theorem do_app_with_code:
@@ -107,6 +108,9 @@ Theorem do_app_Rerr_swap:
           ffi := s1.ffi|> ) = Rerr e
 Proof
   Cases_on `op` \\ rw[do_app_cases_err] \\ rfs[SUBSET_DEF] \\ fs []
+  \\ TRY (strip_tac \\ res_tac \\ fs [])
+  \\ gvs [EXISTS_MEM]
+  \\ last_x_assum $ irule_at Any \\ fs []
   \\ strip_tac \\ res_tac \\ fs []
 QED
 
@@ -118,7 +122,8 @@ Theorem do_app_with_code_err_not_Install:
                          ; compile_oracle := co |>) = Rerr e
 Proof
   rw [Once do_app_cases_err] >> rw [do_app_def] >> fs [SUBSET_DEF] >>
-  fs [do_install_def,case_eq_thms,UNCURRY]
+  fs [do_install_def,case_eq_thms,UNCURRY] >>
+  gvs [EVERY_MEM,EXISTS_MEM]
 QED
 
 Theorem do_app_with_code_err:
@@ -130,6 +135,7 @@ Proof
   fs [do_install_def,case_eq_thms,UNCURRY] >>
   rveq \\ fs [PULL_EXISTS]
   \\ CCONTR_TAC \\ fs []
+  THEN1 gvs [EVERY_MEM,EXISTS_MEM]
   \\ rename1 `s.compile _ args = _`
   \\ qpat_x_assum `args = _` (fn th => fs [GSYM th])
   \\ Cases_on `s.compile (FST (s.compile_oracle 0)) args` \\ fs []
@@ -493,6 +499,7 @@ Proof
   \\ rveq \\ asm_simp_tac (srw_ss()) [do_app_def]
   \\ fs [] \\ every_case_tac \\ fs [] \\ rveq \\ fs []
   \\ fs [do_install_def,UNCURRY] \\ every_case_tac \\ fs [] \\ rw [] \\ fs []
+  \\ gvs [EVERY_MEM,EXISTS_MEM]
 QED
 
 Theorem evaluate_add_clock:
